Rlist.v
@@ -1,0 +1,226 @@
+From Coq Require Import ssreflect FunctionalExtensionality.
+From mathcomp Require Import seq.
+
+Set Bullet Behavior "None".
+Set Implicit Arguments.
+Unset Strict Implicit.
+Unset Printing Implicit Defensive.
+Unset Elimination Schemes.
+
+(* The result of combining the list monad transformer with the reader monad on type R *)
+Inductive Rlist (R : Type) (A : Type) := rnode of (R -> Rnode R A)
+with Rnode (R : Type) (A : Type) := rnil | rcons of A & Rlist R A.
+
+Lemma eq_rnode {R A}:
+  forall f1 f2 : R -> Rnode R A,
+  (forall r, f1 r = f2 r) ->
+  rnode f1 = rnode f2.
+Proof. by move=>?? /functional_extensionality ->. Qed.
+
+Definition t := Rlist.
+
+Arguments rnode [_ _] f.
+Arguments rnil {_ _}.
+Arguments rcons [_ _] x l.
+
+Definition nil {R A} : Rlist R A := rnode (fun _ => rnil).
+Definition cons {R A} (x : R -> A) (l : Rlist R A) : Rlist R A :=
+  rnode (fun r => rcons (x r) l).
+
+Definition lift {R A} (x : A) := @rnode R A (fun _ => rcons x (rnode (fun _ => rnil))).
+
+Fixpoint run {R A} (l : Rlist R A) (r : R) : seq A :=
+  let: rnode n := l in
+  run_node (n r) r
+
+with run_node {R A} (n : Rnode R A) (r : R) : seq A :=
+match n with
+| rnil => [::]
+| rcons x l => x :: run l r
+end.
+
+Fixpoint app {R A} (l1 l2 : Rlist R A) : Rlist R A :=
+  let: rnode n := l1 in
+  rnode (fun r => app_node (n r) l2 r)
+
+with app_node {R A} (n : Rnode R A) (l2 : Rlist R A) : R -> Rnode R A :=
+match n with
+| rnil => fun r => match l2 with rnode n => n r end
+| rcons x l1 => fun r => rcons x (app l1 l2)
+end.
+
+Lemma app_id_r {R A} : forall l : Rlist R A,
+  app l nil = l
+with app_id_r_node {R A} : forall (n : Rnode R A) r,
+  app_node n nil r = n.
+Proof.
+- by case=>?/=; under eq_rnode=>? do rewrite app_id_r_node.
+by case=>//= ???; rewrite app_id_r.
+Qed.
+
+Lemma app_id_l {R A} : forall l : Rlist R A,
+  app nil l = l.
+Proof. by case. Qed.
+
+Lemma app_assoc {R A} : forall l1 l2 l3 : Rlist R A,
+  app l1 (app l2 l3) = app (app l1 l2) l3
+with app_assoc_node {R A} : forall (n1 : Rnode R A) (l2 l3 : Rlist R A) r,
+  app_node n1 (app l2 l3) r = app_node (app_node n1 l2 r) l3 r.
+Proof.
+- by case=>???/=; under eq_rnode=>? do rewrite app_assoc_node.
+case=>/=; first by case.
+by move=>?????; rewrite app_assoc.
+Qed.
+
+Fixpoint map {R A B} (f : A -> B) (l : Rlist R A) : Rlist R B :=
+  let: rnode n := l in
+  rnode (fun r => map_node f (n r))
+with map_node {R A B} (f : A -> B) (n : Rnode R A) :=
+match n with
+| rnil => rnil
+| rcons x l => rcons (f x) (map f l)
+end.
+
+Lemma map_app {R A B}: forall (f : A -> B) (l1 l2 : Rlist R A),
+  map f (app l1 l2) = app (map f l1) (map f l2)
+with map_app_node {R A B}: forall (f : A -> B) (n1 : Rnode R A) l2 r,
+  map_node f (app_node n1 l2 r) = app_node (map_node f n1) (map f l2) r.
+Proof.
+- by move=>?[?]?/=; under eq_rnode=>? do rewrite map_app_node.
+move=>?; case=>/=; first by case.
+by move=>????; rewrite map_app.
+Qed.
+
+Lemma map_map {R A B C} : forall (f : A -> B) (g : B -> C) (l : Rlist R A),
+  map g (map f l) = map (fun x => g (f x)) l
+with map_map_node {R A B C} : forall (f : A -> B) (g : B -> C) (n : Rnode R A),
+  map_node g (map_node f n) = map_node (fun x => g (f x)) n.
+Proof.
+- by move=>??[?]/=; under eq_rnode=>? do rewrite map_map_node.
+move=>??; case=>//=??.
+by rewrite map_map.
+Qed.
+
+Lemma map_id {R A} : forall l : Rlist R A, map id l = l
+with map_id_node {R A} : forall n : Rnode R A, map_node id n = n.
+Proof.
+- by case=>?/=; under eq_rnode=>? do rewrite map_id_node.
+by case=>//=??; rewrite map_id.
+Qed.
+
+Fixpoint set {R S A} (g : S -> R) (l : Rlist R A) : Rlist S A :=
+  let: rnode n := l in
+  rnode (fun r => set_node g (n (g r)))
+with set_node {R S A} (g : S -> R) (n : Rnode R A) :=
+match n with
+| rnil => rnil
+| rcons x l => rcons x (set g l)
+end.
+
+Lemma set_app {R S A} : forall (g : S -> R) (l1 l2 : Rlist R A),
+  set g (app l1 l2) = app (set g l1) (set g l2)
+with set_app_node {R S A} : forall (g : S -> R) (n1 : Rnode R A) l2 r,
+  set_node g (app_node n1 l2 (g r)) = app_node (set_node g n1) (set g l2) r.
+Proof.
+- by move=>?[?]?/=; under eq_rnode=>? do rewrite set_app_node.
+move=>?; case=>/=; first by case.
+by move=>????; rewrite set_app.
+Qed.
+
+Lemma map_set {R S A B} : forall (f : A -> B) (g : S -> R) l,
+  map f (set g l) = set g (map f l)
+with map_set_node {R S A B} : forall (f : A -> B) (g : S -> R) n,
+  map_node f (set_node g n) = set_node g (map_node f n).
+Proof.
+- by move=>??[?]/=; under eq_rnode=>? do rewrite map_set_node.
+move=>??; case=>//=??.
+by rewrite map_set.
+Qed.
+
+Lemma set_set {R S T A} : forall (f : S -> R) (g : T -> S) (l : Rlist R A),
+  set g (set f l) = set (fun r => f (g r)) l
+with set_set_node {R S T A} : forall (f : S -> R) (g : T -> S) (n : Rnode R A),
+  set_node g (set_node f n) = set_node (fun r => f (g r)) n.
+Proof.
+- by move=>??[?]/=; under eq_rnode=>? do rewrite set_set_node.
+move=>??; case=>//=??.
+by rewrite set_set.
+Qed.
+
+Lemma set_id {R A} : forall l : Rlist R A, set id l = l
+with set_id_node {R A} : forall (n : Rnode R A), set_node id n = n.
+Proof.
+- by case=>?/=; under eq_rnode=>? do rewrite set_id_node.
+by case=>//=??; rewrite set_id.
+Qed.
+
+Fixpoint concat {R A} (l : Rlist R (Rlist R A)) : Rlist R A :=
+  let: rnode n := l in
+  rnode (fun r => concat_node (n r) r)
+
+with concat_node {R A} (n : Rnode R (Rlist R A)) : R -> Rnode R A :=
+match n with
+| rnil => fun _ => rnil
+| rcons x l => fun r => let: rnode n := app x (concat l) in n r
+end.
+
+Lemma concat_app {R A} : forall l1 l2 : Rlist R (Rlist R A),
+  concat (app l1 l2) = app (concat l1) (concat l2)
+with concat_app_node {R A} : forall (n1 : Rnode R (Rlist R A)) l2 r,
+  concat_node (app_node n1 l2 r) r = app_node (concat_node n1 r) (concat l2) r.
+Proof.
+- by case=>/=??; under eq_rnode=>? do rewrite concat_app_node.
+case=>/=; case=>? // ???; rewrite concat_app /=.
+by exact: app_assoc_node.
+Qed.
+
+Lemma concat_map {R A} : forall l : Rlist R (Rlist R (Rlist R A)),
+  concat (concat l) = concat (map concat l)
+with concat_map_node {R A} : forall (n : Rnode R (Rlist R (Rlist R A))) r,
+  concat_node (concat_node n r) r = concat_node (map_node concat n) r.
+Proof.
+- by case=>?/=; under eq_rnode=>? do rewrite concat_map_node.
+case=>//=; case=>???.
+rewrite -concat_map /=.
+by exact: concat_app_node.
+Qed.
+
+Lemma map_concat {R A B} : forall (f : A -> B) (l : Rlist R (Rlist R A)),
+  map f (concat l) = concat (map (map f) l)
+with map_concat_node {R A B} : forall (f : A -> B) (n : Rnode R (Rlist R A)) r,
+  map_node f (concat_node n r) = concat_node (map_node (map f) n) r.
+Proof.
+- by move=>?[?]/=; under eq_rnode=>? do rewrite map_concat_node.
+move=>?; case=>//=; case=>???/=.
+by rewrite map_app_node map_concat.
+Qed.
+
+Lemma set_concat {R S A} : forall (g : S -> R) (l : Rlist R (Rlist R A)),
+  set g (concat l) = concat (set g (map (set g) l))
+with set_concat_node {R S A} : forall (g : S -> R) (n : Rnode R (Rlist R A)) r,
+  set_node g (concat_node n (g r)) = concat_node (set_node g (map_node (set g) n)) r.
+Proof.
+- by move=>?[?]/=; under eq_rnode=>? do rewrite set_concat_node.
+move=>?; case=>//=; case=>???/=.
+by rewrite set_app_node set_concat.
+Qed.
+
+Definition collapse {R A} (f : R -> Rlist R A) : Rlist R A :=
+  rnode (fun r => let: rnode n := f r in n r).
+
+Lemma collapse_app {R A} : forall f g : R -> Rlist R A,
+  collapse (fun r => app (f r) (collapse g)) = app (collapse f) (collapse g).
+Proof.
+move=>f ?; rewrite /collapse /=.
+by apply: eq_rnode=>?; case: (f _).
+Qed.
+
+Fixpoint fold_right {R A B} (f : A -> (R -> B) -> (R -> B)) (accu : R -> B) (l : Rlist R A) (r : R) : B :=
+let: rnode n := l in
+fold_right_node f accu (n r) r
+
+with fold_right_node {R A B} (f : A -> (R -> B) -> (R -> B)) (accu : R -> B) (n : Rnode R A) (r : R) : B :=
+match n with
+| rnil => accu r
+| rcons x l => f x (fold_right f accu l) r
+end.
